Fix relativization's database outside contexts

src/Relativization.thy
@@ -105,7 +105,7 @@ signature Relativization =
     val db: (term * term) list
     val init_db : (term * term) list -> theory -> theory
     val get_db : Proof.context -> (term * term) list
-    val relativ_fm: term -> (term * term) list ->  (term * (term * term)) list * Proof.context -> term -> term * (term * (term * term)) list
+    val relativ_fm: term -> (term * term) list ->  (term * (term * term)) list * Proof.context * term option -> term -> term * ((term * (term * term)) list * term list * term list * Proof.context)
     val relativ_tm: term -> (term * term) list ->  (term * (term * term)) list * Proof.context -> term -> term * (term * (term * term)) list * Proof.context
     val read_new_const : Proof.context -> string -> term
     val relativ_tm_frm': term -> (term * term) list -> Proof.context -> term -> term option * term
@@ -155,10 +155,14 @@ structure Data = Generic_Data
      {db_rels = AList.join (op aconv) (K #1) (db', db)};
 );
 
-fun init_db db = Context.theory_map (Data.put {db_rels = db })
-fun get_db thy = let val db = Data.get (Context.Proof thy)
-                 in #db_rels db
-                 end
+fun init_db db = Context.theory_map (Data.put {db_rels = db})
+
+fun get_db thy =
+  let
+    val db = Data.get (Context.Proof thy)
+ in
+    #db_rels db
+end
 
 val read_const = Proof_Context.read_const {proper = true, strict = true}
 val read_new_const = Proof_Context.read_term_pattern
@@ -169,7 +173,7 @@ fun add_rel_const thm_name c t ctxt (rs as {db_rels = db}) =
     (warning ("Ignoring duplicate relativization rule" ^
               const_name c ^ " " ^ Syntax.string_of_term ctxt t ^
               "(" ^  Syntax.string_of_term ctxt t' ^ " in " ^ thm_name ^ ")"); rs)
-  | NONE => {db_rels = (c, t) :: db};
+  | NONE => {db_rels = (c, t) :: db}
 
 fun get_consts thm =
   let val (c_rel, rhs) = Thm.concl_of thm |> Utils.dest_trueprop |>
@@ -187,10 +191,13 @@ end
 
 
 fun add_constant rel abs thy =
-  let val c_abs = read_new_const thy abs
-      val c_rel = read_new_const thy rel
-  in Local_Theory.target (Context.proof_map
-    (Data.map (fn db => {db_rels = (c_rel,c_abs) :: #db_rels db}))) thy
+  let
+    val c_abs = read_new_const thy abs
+    val c_rel = read_new_const thy rel
+    fun add_to_context ctxt' = Context.proof_map (Data.map (fn db => {db_rels = (c_rel,c_abs) :: #db_rels db})) ctxt'
+    fun add_to_theory ctxt' = Local_Theory.raw_theory (Context.theory_map (Data.map (fn db => {db_rels = (c_rel,c_abs) :: #db_rels db}))) ctxt'
+  in
+    Local_Theory.target (add_to_theory o add_to_context) thy
  end
 
 fun del_rel_const c (rs as {db_rels = db}) =
@@ -230,6 +237,14 @@ val absolute_rels = [ @{const ZF_Base.mem}
                     , @{const True}
                     , @{const False}
                     ]
+
+infix 6 @@
+fun op @@ (xs, ys) = union (op =) ys xs
+
+fun concatt xss = fold (curry op @@) xss []
+
+infix 6 &&&
+fun op &&& (f, g) = fn x => (f x, g x)
 
 (* Creates the relational term corresponding to a term of type i. If the last
   argument is (SOME v) then that variable is not bound by an existential
@@ -272,42 +287,46 @@ and
             in (v, r_tm, ctxt1)
             end
         | NONE => raise TERM ("Constant " ^ const_name c ^ " is not present in the db." , nil)
-
       (* relativization of a partially applied constant *)
-      fun relativ_app tm abs_args (Const c) args rs =
-            let val (w_ts, rs_ts, ctxt_ts) = relativ_tms pred rel_db rs ctxt args
-                val (w_tm, r_tm, ctxt_tm) = mk_rel_const (Const c) w_ts abs_args ctxt_ts
-                val rs_ts' = update_tm (tm, (w_tm, r_tm)) rs_ts
-            in (w_tm, rs_ts', ctxt_tm)
+      fun relativ_app ctxt' tm abs_args (Const c) args rs =
+            let
+              val (w_ts, rs_ts, ctxt_ts) = relativ_tms pred rel_db rs (the_default ctxt ctxt') args
+              val (w_tm, r_tm, ctxt_tm) = mk_rel_const (Const c) w_ts abs_args ctxt_ts
+              val rs_ts' = update_tm (tm, (w_tm, r_tm)) rs_ts
+            in
+              (w_tm, rs_ts', ctxt_tm)
             end
-        | relativ_app _ _ t _ _ =
+        | relativ_app _ _ _ t _ _ =
             raise TERM ("Tried to relativize an application with a non-constant in head position",[t])
 
       (* relativization of non dependent product and sum *)
       fun relativ_app_no_dep tm c t t' rs =
           if loose_bvar1 (t', 0)
           then raise TERM("A dependency was found when trying to relativize", [tm])
-          else relativ_app tm [] c [t, incr_boundvars ~1 t'] rs
+          else relativ_app NONE tm [] c [t, incr_boundvars ~1 t'] rs
 
       fun go (Var _) = raise TERM ("Var: Is this possible?",[])
-        | go (@{const Replace} $ t $ pc) =
-            let val (pc', rs') = relativ_fm pred rel_db (rs, ctxt) pc
-            in relativ_app tm [pc'] @{const Replace} [t] rs'
+        | go (@{const Replace} $ t $ Abs body) =
+            let
+              val (v, b) = Term.dest_abs body |>> var_i
+              val (b', (rs', ctxt')) = relativ_fm pred rel_db (rs, ctxt, SOME v) b ||> #1 &&& #4
+            in
+              relativ_app (SOME ctxt') tm [lambda v b'] @{const Replace} [t] rs'
             end
         | go (@{const Collect} $ t $ pc) =
-            let val (pc', rs') = relativ_fm pred rel_db (rs,ctxt) pc
-            in relativ_app tm [pc'] @{const Collect} [t] rs'
+            let val (pc', (rs', ctxt')) = relativ_fm pred rel_db (rs,ctxt, NONE) pc ||> #1 &&& #4
+            in relativ_app (SOME ctxt') tm [pc'] @{const Collect} [t] rs'
             end
         | go (tm as @{const Sigma} $ t $ Abs (_,_,t')) =
             relativ_app_no_dep tm @{const Sigma} t t' rs
         | go (tm as @{const Pi} $ t $ Abs (_,_,t')) =
             relativ_app_no_dep tm @{const Pi} t t' rs
         | go (tm as @{const bool_of_o} $ t) =
-            let val (t', rs') = relativ_fm pred rel_db (rs, ctxt) t
-            in relativ_app tm [t'] @{const bool_of_o} [] rs'
+            let val (t', (rs', ctxt')) = relativ_fm pred rel_db (rs, ctxt, NONE) t ||> #1 &&& #4
+            in relativ_app (SOME ctxt') tm [t'] @{const bool_of_o} [] rs'
             end
-        | go (tm as Const _) = relativ_app tm [] tm [] rs
-        | go (tm as _ $ _) = (strip_comb tm |> uncurry (relativ_app tm [])) rs
+        | go (tm as Const _) = relativ_app NONE tm [] tm [] rs
+        | go (tm as _ $ _) = (strip_comb tm |> uncurry (relativ_app NONE tm [])) rs
         | go tm = (tm, update_tm (tm,(tm,tm)) rs, ctxt)
 
       (* we first check if the term has been already relativized as a variable *)
@@ -316,7 +335,7 @@ and
          | SOME (w, _) => (w, rs, ctxt)
       end
 and
-  relativ_fm pred rel_db (rs,ctxt) fm =
+  relativ_fm pred rel_db (rs, ctxt, v) fm =
   let
 
   (* relativization of a fully applied constant *)
@@ -338,11 +357,6 @@ and
   infix 6 --
   fun op -- (xs, ys) = subtract (op =) ys xs
 
-  infix 6 @@
-  fun op @@ (xs, ys) = union (op =) ys xs
-
-  fun concatt xss = fold (curry op @@) xss []
-
   fun reachable p u xs =
     let
       val step = map (fn x => filter (p x) (u -- xs)) xs |> concatt
@@ -358,33 +372,29 @@ and
     let
       fun contains_b0 t = loose_bvar1 (t, 0)
 
+      fun contains_extra_var t =
+        case v of
+          SOME v => fold_aterms (fn t => fn acc => t = v orelse acc) t false
+        | NONE => false
+
+      fun contains_b0_extra t = contains_b0 t orelse contains_extra_var t
+
       (* t1 $ v \<hookrightarrow> t2 iff v \<in> FV(t2) *)
       fun chained_frees (_ $ v) t2 = Utils.inList (get_frees t2) v
         | chained_frees t _ = raise TERM ("Malformed term", [t])
 
-      val tms_to_close = filter contains_b0 tms |> reachable chained_frees tms
+      val tms_to_close = filter contains_b0_extra tms |> reachable chained_frees tms
       val tms_to_keep = map (incr_boundvars ~1) (tms -- tms_to_close)          
       val vars_to_close = inter (op =) (map (List.last o #2 o strip_comb) tms_to_close) vars
       val vars_to_keep = vars -- vars_to_close
       val new_rs =
         rs
-        |> filter (fn (k, (v, rel)) => not (contains_b0 k orelse contains_b0 v orelse contains_b0 rel))
+        |> filter (fn (k, (v, rel)) => not (contains_b0_extra k orelse contains_b0_extra v orelse contains_b0_extra rel))
         |> map (fn (k, (v, rel)) => (incr_boundvars ~1 k, (incr_boundvars ~1 v, incr_boundvars ~1 rel)))
     in
       (fold (fn v => fn t => rex pred (incr_boundvars 1 t) v) vars_to_close (conjs (f :: tms_to_close)),
        (new_rs, vars_to_keep, tms_to_keep, ctxt))
     end
-
-  fun finally_close_fm (f, (rs, vars, tms, ctxt)) =
-    (fold (fn  v => fn t => rex pred (incr_boundvars 1 t) v) vars (conjs (f :: tms)), (rs, [], [], ctxt))
-
-  fun get_bounds (l as Abs _) = op @@ (strip_abs l |>> map (op #1) ||> get_bounds)
-    | get_bounds (t as _$_) = strip_comb t |> op :: |> map get_bounds |> concatt
-    | get_bounds _ = []
-
-  fun update_ctxt v c = if Variable.is_fixed c v then c else #2 (Variable.add_fixes [v] c)
-
-  val initial_ctxt = fold update_ctxt (get_bounds fm) ctxt
 
   (* Handling of bounded quantifiers. *)
   fun bquant (ctxt, rs) quant conn dom pred =
@@ -419,19 +429,37 @@ and
         go (ctxt, new_rs) t |> close_fm |>> lambda (var_i v)
       end
     | go _ t = raise TERM ("Relativization of formulas cannot handle this case.",[t])
-  in go (initial_ctxt, rs) fm |> finally_close_fm ||> #1
+  in
+    go (ctxt, rs) fm
   end
 
 
 fun relativ_tm_frm' cls_pred db ctxt tm =
-  let val ty = fastype_of tm
-  in case ty of
+  let
+    fun get_bounds (l as Abs _) = op @@ (strip_abs l |>> map (op #1) ||> get_bounds)
+      | get_bounds (t as _$_) = strip_comb t |> op :: |> map get_bounds |> concatt
+      | get_bounds _ = []
+
+    fun update_ctxt v c = if Variable.is_fixed c v then c else #2 (Variable.add_fixes [v] c)
+
+    val ty = fastype_of tm
+    val initial_ctxt = fold update_ctxt (get_bounds tm) ctxt
+  in
+    case ty of
         @{typ i} =>
-          let val (w, rs, _) =  relativ_tm cls_pred db ([],ctxt) tm
-          in (SOME w, close_rel_tm cls_pred NONE (SOME w) rs)
+          let
+            val (w, rs, _) =  relativ_tm cls_pred db ([], initial_ctxt) tm
+          in
+            (SOME w, close_rel_tm cls_pred NONE (SOME w) rs)
           end
-      | @{typ o} => (NONE, #1 (relativ_fm cls_pred db ([],ctxt) tm))
-      | ty' => raise TYPE ("We can relativize only terms of types i and o",[ty'],[tm])
+      | @{typ o} =>
+          let
+            fun close_fm (f, (_, vars, tms, _)) =
+              fold (fn  v => fn t => rex cls_pred (incr_boundvars 1 t) v) vars (conjs (f :: tms))
+          in
+            (NONE, relativ_fm cls_pred db ([], initial_ctxt, NONE) tm |> close_fm)
+          end
+      | ty' => raise TYPE ("We can relativize only terms of types i and o", [ty'], [tm])
   end
 
 fun lname ctxt = Local_Theory.full_name ctxt o Binding.name
@@ -449,14 +477,14 @@ fun relativize_def def_name thm_ref pos lthy =
     val vs = cls_pred :: map (Thm.term_of o #2) vs' @ the_list v
     val at = List.foldr (uncurry lambda) t vs
     val abs_const = read_const lthy (lname lthy thm_ref)
-in
-   lthy |>
-   Local_Theory.define ((Binding.name def_name, NoSyn),
-                         ((Binding.name (def_name ^ "_def"), []), at)) |>>
-   (#2 #> (fn (s,t) => (s,[t]))) |> Utils.display "theorem" pos |>
-   Local_Theory.target (
-       fn ctxt' => Context.proof_map
-        (Data.map (add_rel_const "" abs_const (read_new_const ctxt' def_name) ctxt')) ctxt')
+    fun add_to_context ctxt' = Context.proof_map (Data.map (add_rel_const "" abs_const (read_new_const ctxt' def_name) ctxt')) ctxt'
+    fun add_to_theory ctxt' = Local_Theory.raw_theory (Context.theory_map (Data.map (add_rel_const "" abs_const (read_new_const ctxt' def_name) ctxt'))) ctxt'
+  in
+    lthy
+    |> Local_Theory.define ((Binding.name def_name, NoSyn), ((Binding.name (def_name ^ "_def"), []), at))
+    |>> (#2 #> (fn (s,t) => (s,[t])))
+    |> Utils.display "theorem" pos
+    |> Local_Theory.target (add_to_theory o add_to_context)
   end
 
 fun relativize_tm def_name term pos lthy =
@@ -471,13 +499,12 @@ fun relativize_tm def_name term pos lthy =
     val (v,t) = relativ_tm_frm' cls_pred db' ctxt2 tm
     val vs = cls_pred :: map Free vs' @ the_list v
     val at = List.foldr (uncurry lambda) t vs
-in
-   lthy |>
-    Local_Theory.define ((Binding.name def_name, NoSyn),
-                        ((Binding.name (def_name ^ "_def"), []), at)) |>>
-  (#2 #> (fn (s,t) => (s,[t]))) |> Utils.display "theorem" pos
+  in
+    lthy
+    |> Local_Theory.define ((Binding.name def_name, NoSyn), ((Binding.name (def_name ^ "_def"), []), at))
+    |>> (#2 #> (fn (s,t) => (s,[t])))
+    |> Utils.display "theorem" pos
   end
-
 
 end
 \<close>
@@ -491,7 +518,6 @@ local
      Outer_Syntax.local_theory \<^command_keyword>\<open>reldb_add\<close> "ML setup for adding relativized/absolute pairs"
        (relativize_parser >> (fn ((rel_term,abs_term),_) =>
           Relativization.add_constant rel_term abs_term))
-
 
   val _ =
      Outer_Syntax.local_theory \<^command_keyword>\<open>relativize\<close> "ML setup for relativizing definitions"
