src/Relativization_Test.thy
@@ -62,6 +62,8 @@ definition "test7" :: "i \<Rightarrow> o" where
 
 relativize "test7" "is_test7"
 
+relativize_tm "test7(0)" "is_testt7"
+
 definition "test8" :: "o" where
   "test8 \<equiv> \<forall> a . test7(a)"
 
@@ -109,10 +111,82 @@ relativize_tm "\<forall> a . 0 \<subseteq> a" "test15"
 
 relativize_tm "\<forall> a . a = <a,0>" "test16"
 
+definition "between" :: "i \<Rightarrow> i \<Rightarrow> i \<Rightarrow> o" where
+  "between(x, a, b) \<equiv> a \<subseteq> x \<and> x \<subseteq> b"
+
+relativize "between" "is_between"
+
+lemma (in M_trans) "between_ok":
+  "\<forall> a b x . M(a) \<and> M(b) \<and> M(c) \<Longrightarrow> between(x, a, b) \<longleftrightarrow> is_between(M, x, a, b)"
+  unfolding between_def is_between_def
+  using subset_abs
+  by simp
+
+definition "covered_by" :: "i \<Rightarrow> i \<Rightarrow> o" where
+  "covered_by(a, b) \<equiv> a \<subseteq> b \<and> (\<forall> x . between(x, a, b) \<longrightarrow> x = a \<or> x = b)"
+
+relativize "covered_by" "is_covered_by"
+
+lemma (in M_trans) "covered_by_ok":
+  "\<forall> a b . M(a) \<and> M(b) \<Longrightarrow> covered_by(a, b) \<longleftrightarrow> is_covered_by(M, a, b)"
+  unfolding covered_by_def is_covered_by_def
+  using between_ok
+  by auto
+
+definition "min_elem" :: "i \<Rightarrow> i \<Rightarrow> o" where
+  "min_elem(u, m) \<equiv> m \<in> u \<and> (\<forall> x . x \<in> u \<longrightarrow> m \<subseteq> x)"
+
+relativize "min_elem" "is_min_elem"
+
+lemma (in M_trans) "min_elem_ok":
+  "\<forall> u m . M(u) \<and> M(m) \<Longrightarrow> min_elem(u, m) \<longleftrightarrow> is_min_elem(M, u, m)"
+  unfolding min_elem_def is_min_elem_def
+  using subset_abs
+  by auto
+
+definition "atoms" :: "i \<Rightarrow> i" where
+  "atoms(u) \<equiv> { a \<in> u . \<exists> m . min_elem(u, m) \<and> covered_by(m, a) }"
+
+relativize "atoms" "is_atoms"
+
+lemma (in M_trans) "unique_atoms":
+  "\<forall> u a b . M(u) \<and> M(a) \<and> M(b) \<Longrightarrow> is_atoms(M, u, a) \<and> is_atoms(M, u, b) \<longrightarrow> a = b"
+  unfolding is_atoms_def
+  using covered_by_ok min_elem_ok
+  by simp
+
+lemma (in M_trans) "atoms_ok":
+  "\<forall> u . M(u) \<Longrightarrow> is_atoms(M, u, atoms(u))"
+  unfolding atoms_def is_atoms_def
+  using covered_by_ok min_elem_ok
+  by auto
+
+lemma (in M_trans) "atoms_abs":
+  "\<forall> u a . M(u) \<and> M(a) \<Longrightarrow> a = atoms(u) \<longleftrightarrow> is_atoms(M, u, a)"
+  using unique_atoms atoms_ok
+  by blast
+
+relativize_tm "{ a : u . <0,0> \<in> a } \<inter> { b : u . 0 \<in> b }" "test17"
+
+relativize_tm "{ b . f \<in> x \<rightarrow> y, \<forall> x . \<exists> a . f ` (f ` x) = f ` x \<and>  f ` a = b }" "test18"
+
 (* collect { a \<in> 0 . a=a} *)
 (* rep_fun { a. <a,b>\<in>0 } *)
 (* replace { a. a\<in>0, a=a } *)
 (*         { b. a\<in>0, b=a\<times>a } *)
 (* RepFun { a\<times>a. a\<in>0 } *)
+
+(*
+ML\<open>
+Local_Theory.target I @{context}
+\<close>
+*)
+
+context M_trans
+begin
+ML\<open>
+Local_Theory.target I @{context}
+\<close>
+end
 
 end
